![[Notas gu√≠a 1#^ldpn9ytbd3]]

| $+$        | $\alpha$ | $\beta$  | $\gamma$ | $\delta$ |
| -------- | -------- | -------- | -------- | -------- |
| $\alpha$ | $\alpha$ | $\beta$  | $\gamma$ | $\delta$ |
| $\beta$  | $\beta$  | $\beta$  | $\delta$ | $\delta$ |
| $\gamma$ | $\gamma$ | $\delta$ | $\gamma$ | $\delta$ |
| $\delta$ | $\delta$ | $\delta$ | $\delta$ | $\delta$ | 

| $\cdot$  | $\alpha$ | $\beta$  | $\gamma$ | $\delta$ |
| -------- | -------- | -------- | -------- | -------- |
| $\alpha$ | $\alpha$ | $\alpha$ | $\alpha$ | $\alpha$ |
| $\beta$  | $\alpha$ | $\beta$  | $\alpha$ | $\beta$  |
| $\gamma$ | $\alpha$ | $\alpha$ | $\gamma$ | $\gamma$ |
| $\delta$ | $\alpha$ | $\beta$  | $\gamma$ | $\delta$ | 



![[hass ejer32|200x300]]


$$
\left\{
\begin{split}
\alpha + w \cdot (x +y+z) &= \delta \\
\delta \cdot x\cdot y +x \cdot z+\alpha &=y\cdot w \\
\beta \cdot \gamma \cdot z + x\cdot y\cdot w +\alpha\delta &= \alpha\gamma

\end{split}
\right.
$$


$$
\left\{
\begin{split}
0 + w \cdot (x +y+z) &= \delta \\
1 \cdot x\cdot y +x \cdot z+0 &=y\cdot w \\
\cancelto{ 0 }{ \gamma' \cdot \gamma } \cdot z + x\cdot y\cdot w + 0\cdot 1 &= 0\cdot \gamma

\end{split}
\right.
$$
$\implies w=1 \ \wedge x'=z \wedge z' =x\wedge0=y$

